Add missing wf conditions to definitions

CCsub_Definitions.v
@@ -666,12 +666,14 @@ Inductive typing : env -> sig -> exp -> typ -> Prop :=
   | typing_handle : forall L E Q T1 e,
       (forall x : atom, x `notin` L ->
         ([(x, bind_typ (typ_capt {*} (typ_ret T1)))] ++ E) @ Q |-t (open_ee e x (`cset_fvar` x)) ~: T1) ->
+      wf_typ_in E T1 ->
       ~ (E |-sc {*} <: (cv T1)) ->
       E @ Q |-t (exp_handle T1 e) ~: T1
 
   | typing_do_ret : forall E Q C T1 T2 e1 e2,
       E @ Q |-t e1 ~: (typ_capt C (typ_ret T1)) ->
       E @ Q |-t e2 ~: T1 ->
+      wf_typ_in E T2 ->
       E @ Q |-t (exp_do_ret e1 e2) ~: T2
 
   | typing_lvar : forall E Q C T l,
